Phi_Semantics/PhiSem_CF_Breakable.thy
@@ -12,14 +12,14 @@ proc while:
                   \<^bold>p\<^bold>r\<^bold>o\<^bold>c Cond \<lbrace> X x \<longmapsto> X x'\<heavy_comma> \<^bold>v\<^bold>a\<^bold>l cond x' \<Ztypecolon> \<bool> \<^bold>s\<^bold>u\<^bold>b\<^bold>j x'. invariant x' \<rbrace> \<^bold>t\<^bold>h\<^bold>r\<^bold>o\<^bold>w\<^bold>s E1"
   and B: "\<And>x lb lc. \<^bold>p\<^bold>r\<^bold>e\<^bold>m\<^bold>i\<^bold>s\<^bold>e invariant x \<Longrightarrow>
                     \<^bold>p\<^bold>r\<^bold>e\<^bold>m\<^bold>i\<^bold>s\<^bold>e cond x \<Longrightarrow>
-                    break_\<phi>app\<^bold>:
+                    break_\<phi>app\<^bold>: HIDDEN_PREM(
                         \<^bold>p\<^bold>r\<^bold>o\<^bold>c (op_break lb \<phi>V_none :: unit proc)
                            \<lbrace> (X x'\<heavy_comma> Brk_Frame lc \<^bold>s\<^bold>u\<^bold>b\<^bold>j x'. invariant x' \<and> \<not> cond x')\<heavy_comma> Brk_Frame lb \<longmapsto> 0 \<rbrace>
-                        \<^bold>t\<^bold>h\<^bold>r\<^bold>o\<^bold>w\<^bold>s (\<lambda>_. Brking_Frame lb (\<lambda>_::unit \<phi>arg. X x'\<heavy_comma> Brk_Frame lc \<^bold>s\<^bold>u\<^bold>b\<^bold>j x'. invariant x' \<and> \<not> cond x')) \<Longrightarrow>
-                    continue_\<phi>app\<^bold>:
+                        \<^bold>t\<^bold>h\<^bold>r\<^bold>o\<^bold>w\<^bold>s (\<lambda>_. Brking_Frame lb (\<lambda>_::unit \<phi>arg. X x'\<heavy_comma> Brk_Frame lc \<^bold>s\<^bold>u\<^bold>b\<^bold>j x'. invariant x' \<and> \<not> cond x'))) \<Longrightarrow>
+                    continue_\<phi>app\<^bold>: HIDDEN_PREM(
                         \<^bold>p\<^bold>r\<^bold>o\<^bold>c (op_break lc \<phi>V_none :: unit proc)
                            \<lbrace> (X x'\<heavy_comma> Brk_Frame lb \<^bold>s\<^bold>u\<^bold>b\<^bold>j x'. invariant x')\<heavy_comma> Brk_Frame lc \<longmapsto> 0 \<rbrace>
-                        \<^bold>t\<^bold>h\<^bold>r\<^bold>o\<^bold>w\<^bold>s (\<lambda>_. Brking_Frame lc (\<lambda>_::unit \<phi>arg. X x'\<heavy_comma> Brk_Frame lb \<^bold>s\<^bold>u\<^bold>b\<^bold>j x'. invariant x')) \<Longrightarrow>
+                        \<^bold>t\<^bold>h\<^bold>r\<^bold>o\<^bold>w\<^bold>s (\<lambda>_. Brking_Frame lc (\<lambda>_::unit \<phi>arg. X x'\<heavy_comma> Brk_Frame lb \<^bold>s\<^bold>u\<^bold>b\<^bold>j x'. invariant x'))) \<Longrightarrow>
                     \<^bold>p\<^bold>r\<^bold>o\<^bold>c Body lb lc
                         \<lbrace> X x\<heavy_comma> Brk_Frame lc\<heavy_comma> Brk_Frame lb
                       \<longmapsto> X x'\<heavy_comma> Brk_Frame lc\<heavy_comma> Brk_Frame lb \<^bold>s\<^bold>u\<^bold>b\<^bold>j x'. invariant x'
@@ -35,8 +35,8 @@ proc while:
       \<medium_left_bracket> C \<medium_right_bracket>.
       \<medium_left_bracket> brk_scope \<medium_left_bracket> for lc
           B[where lb1=lb]
-          "_op_break_rule_"[THEN Labelled_I]
-          "_op_break_rule_"[THEN Labelled_I]
+          "_op_break_rule_"[THEN HIDDEN_PREM_I, THEN Labelled_I]
+          "_op_break_rule_"[THEN HIDDEN_PREM_I, THEN Labelled_I]
         \<medium_right_bracket> for \<open>(X x'\<heavy_comma> Brk_Frame lb \<^bold>s\<^bold>u\<^bold>b\<^bold>j x'. invariant x')\<heavy_comma> Brk_Frame lc\<close> .. ;;
       \<medium_right_bracket>. ;;
     \<medium_right_bracket> for \<open>(X x' \<^bold>s\<^bold>u\<^bold>b\<^bold>j x'. invariant x' \<and> \<not> cond x')\<heavy_comma> Brk_Frame lb\<close> .. ;;
