Phi_Semantics/PhiSem_Play_Ground.thy
@@ -35,6 +35,8 @@ proc
 setup \<open>Context.theory_map (Generic_Variable_Access.Process_of_Argument.put
            (SOME Generic_Variable_Access.to_value_no_clean))\<close> *)
 
+(* declare [[\<phi>hide_techinicals=false]] *)
+
 proc
   input \<open>\<^bold>v\<^bold>a\<^bold>l x \<Ztypecolon> \<nat>[32]\<close>
   premises \<open>x < 10\<close>
